theories/Coherence/Coherence.v
@@ -162,51 +162,154 @@ Proof.
 Qed.
 
 
-(*
+
 (** *** In a coherent program, the globals of every function that can eventually be called are live *)
 
+Lemma srd_globals_live_F ZL Lv F als f lv' Z' l DL
+      (LEN1 : ❬F❭ = ❬als❭) (Len2:❬ZL❭=❬Lv❭) (Len3:❬ZL❭=❬DL❭)
+      (IH : forall k Zs, get F k Zs ->
+                    forall (ZL : 〔params〕) (Lv : 〔⦃var⦄〕) (DL : 〔؟ ⦃var⦄〕) (alv : ann ⦃var⦄) (f : lab),
+                      live_sound Imperative ZL Lv (snd Zs) alv ->
+                      srd DL (snd Zs) alv ->
+                      PIR2 (ifFstR Equal) DL (Lv \\ ZL) ->
+                      isCalled (snd Zs) f ->
+                      ❬ZL❭ = ❬Lv❭ ->
+                      ❬ZL❭ = ❬DL❭ ->
+                      exists (lv : ⦃var⦄) (Z : params), get ZL f Z /\ get DL f ⎣ lv ⎦ /\ lv ⊆ getAnn alv)
+      (LS: forall (n : nat) (Zs : params * stmt) (a : ann ⦃var⦄),
+          get F n Zs ->
+          get als n a ->
+          live_sound Imperative (fst ⊝ F ++ ZL) (getAnn ⊝ als ++ Lv) (snd Zs) a)
+      (SRD: forall (n : nat) (Zs : params * stmt) (a : ann ⦃var⦄),
+          get F n Zs ->
+          get als n a ->
+          srd (restr (getAnn a \ of_list (fst Zs)) ⊝ (Some ⊝ (getAnn ⊝ als) \\ (fst ⊝ F) ++ DL))
+              (snd Zs) a)
+      (PE:PIR2 (ifFstR Equal) (Some ⊝ (getAnn ⊝ als) \\ (fst ⊝ F) ++ DL)
+               ((getAnn ⊝ als ++ Lv) \\ (fst ⊝ F ++ ZL)))
+      (CC:callChain isCalled F l f)
+      (GetZL : get (fst ⊝ F ++ ZL) l Z')
+      (GetLv : get (getAnn ⊝ als ++ Lv) l lv')
+      dv (GetDL : get (Some ⊝ (getAnn ⊝ als) \\ (fst ⊝ F) ++ DL) l ⎣ dv ⎦)
+      (dvEq:dv [=] lv' \ of_list Z')
+  : exists (lv : ⦃var⦄) (Z : params) dv,
+    get (fst ⊝ F ++ ZL) (labN f) Z
+    /\ get (getAnn ⊝ als ++ Lv) (labN f) lv
+    /\ get (restr (lv \ of_list Z) ⊝ (Some ⊝ (getAnn ⊝ als) \\ (fst ⊝ F) ++ DL)) (labN f) (Some dv)
+    /\ dv [=] (lv \ of_list Z) /\ lv \ of_list Z ⊆ lv' \ of_list Z'.
+Proof.
+  general induction CC.
+  - do 2 eexists; eexists (dv); split; [| split; [|split]]; eauto.
+    eapply map_get_eq; eauto using zip_get, map_get_1.
+    simpl; cases; eauto. eauto. exfalso. apply NOTCOND; rewrite dvEq; eauto.
+  - inv_get.
+    assert (Incl:(of_list (fst Zs)) ⊆ (list_union ((fun Zs : params * stmt => of_list (fst Zs) ∪ definedVars (snd Zs)) ⊝ F))). {
+      eapply incl_list_union; eauto using map_get_1.
+    }
+    exploit (IH k Zs); eauto using restrict_ifFstR; [ eauto with len | eauto with len |].
+    dcr.
+    edestruct (@get_length_eq _ _ (fst ⊝ F ++ ZL) (getAnn ⊝ als ++ Lv)); eauto.
+    eauto with len. inv_get.
+    PIR2_inv; inv_get.
+    exploit IHCC; try eapply H4; eauto.
+    eapply get_app_cases in H3. destruct H3; dcr; inv_get.
+    + do 3 eexists; split; [| split; [|split] ]; eauto.
+      eapply map_get_eq. eauto. simpl. cases; eauto.
+      split; eauto.
+      rewrite <- H5. rewrite <- H14. eauto.
+    + do 2 eexists; eexists x5; split; [| split ]; eauto.
+      assert (Len4:❬Some ⊝ (getAnn ⊝ als) \\ (fst ⊝ F)❭ = ❬F❭) by eauto with len.
+      rewrite get_app_ge in H1; eauto with len.
+      rewrite get_app_ge in H4; rewrite Len4, map_length, <- LEN1 in *; eauto.
+      inv_get. split.
+      eapply map_get_eq; eauto. simpl; cases; eauto.
+      split; eauto.
+      rewrite <- H5, H9. eauto.
+      rewrite map_length in *; rewrite  <- LEN1; eauto.
+Qed.
+
 Lemma srd_globals_live s ZL Lv DL alv f
-: live_sound Imperative ZL Lv s alv
-  -> srd DL s alv
-  -> PIR2 (ifFstR Equal) DL (Lv \\ ZL)
-  -> isCalled s f
-  -> exists lv Z, get ZL (counted f) Z
+  (LS:live_sound Imperative ZL Lv s alv)
+  (SRD:srd DL s alv)
+  (PE:PIR2 (ifFstR Equal) DL (Lv \\ ZL))
+  (IC:isCalled s f)
+  (Len1:❬ZL❭=❬Lv❭) (Len2:❬ZL❭=❬DL❭)
+  : exists lv Z, get ZL (counted f) Z
             /\ get DL (counted f) (Some lv)
             /\ lv ⊆ getAnn alv.
 Proof.
-  intros LS SRD PE IC.
-  general induction IC; try invt live_sound; try invt srd; simpl in * |- *.
-  - edestruct IHIC as [lv' [Z' ?]]; eauto using restrict_ifFstR; dcr.
+  revert_except s.
+  sind s.
+  intros.
+  invt live_sound; invt srd; invt isCalled; simpl in * |- *.
+  - edestruct (IH s0) as [lv' [Z' ?]]; eauto using restrict_ifFstR; dcr.
     inv_get.
     do 2 eexists; split; [| split]. eauto. eauto.
-
-    idtac "improve". rewrite H. eauto with cset.
-  - edestruct IHIC; eauto; dcr; inv_get. eauto with cset.
-  - edestruct IHIC; eauto; dcr; inv_get. eauto with cset.
+    idtac "improve". rewrite H3. eauto with cset.
+  - edestruct (IH s1); eauto; dcr; inv_get. eauto with cset.
+  - edestruct (IH s2); eauto; dcr; inv_get. eauto with cset.
   - PIR2_inv. inv_get.
     do 2 eexists; split; [| split]; eauto with cset.
-    idtac "improve"; rewrite H5; eauto.
-  - edestruct IHIC; eauto using restrict_ifFstR; dcr; inv_get.
-    do 2 eexists; split; [| split]; eauto.
-    rewrite H. eauto with cset.
-  - inv_get.
-    edestruct IHIC2; eauto.
+    idtac "improve"; rewrite H7; eauto.
+  - assert (PIR2 (ifFstR Equal) (Some ⊝ (getAnn ⊝ als) \\ (fst ⊝ F) ++ DL)
+                 ((getAnn ⊝ als) \\ (fst ⊝ F) ++ Lv \\ ZL)). {
+      eapply PIR2_app; eauto using restrict_ifFstR, PIR2_ifFstR_refl.
+    }
+    edestruct (IH t); eauto with len. rewrite zip_app; eauto with len.
+    destruct l'; simpl in *; dcr; inv_get.
+    edestruct PIR2_nth; eauto; dcr. invc H13.
+    edestruct (@get_length_eq _ _ (fst ⊝ F ++ ZL) (getAnn ⊝ als ++ Lv)); eauto.
+    eauto with len.
+    rewrite <- zip_app in H9; eauto with len. inv_get.
+    exploit srd_globals_live_F; eauto using restrict_ifFstR.
+    intros; eapply (IH (snd Zs)); eauto.
+    rewrite zip_app; eauto with len.
+    dcr; destruct f; simpl in *; inv_get.
+    do 2 eexists; split; [|split]; eauto.
+    rewrite <- H3, <- H14, H15, H18. eauto.
+Qed.
+
+
+Lemma srd_globals_live_From ZL Lv DL s F als f alv
+      (ICF:isCalledFrom isCalled F s f)
+      (LS:live_sound Imperative (fst ⊝ F ++ ZL) (getAnn ⊝ als ++ Lv) s alv)
+      (SRD:srd ((Some ⊝ (getAnn ⊝ als) \\ (fst ⊝ F) ++ DL)) s alv)
+      (Len1 : ❬F❭ = ❬als❭)
+      (Len2 : ❬ZL❭ = ❬Lv❭)
+      (Len3 : ❬ZL❭ = ❬DL❭)
+      (LSF: forall (n : nat) (Zs : params * stmt) (a : ann ⦃var⦄),
+          get F n Zs ->
+          get als n a ->
+          live_sound Imperative (fst ⊝ F ++ ZL) (getAnn ⊝ als ++ Lv) (snd Zs) a)
+      (SRDF: forall (n : nat) (Zs : params * stmt) (a : ann ⦃var⦄),
+          get F n Zs ->
+          get als n a ->
+          srd (restr (getAnn a \ of_list (fst Zs)) ⊝ (Some ⊝ (getAnn ⊝ als) \\ (fst ⊝ F) ++ DL))
+              (snd Zs) a)
+      (PE:PIR2 (ifFstR Equal) DL (Lv \\ ZL))
+
+  : exists (lv : ⦃var⦄) (Z : params),
+    get (fst ⊝ F ++ ZL) (labN f) Z /\
+    get (getAnn ⊝ als ++ Lv) (labN f) lv
+    /\ (lv \ of_list Z) ⊆ getAnn alv.
+Proof.
+  destruct ICF as [? [IC CC]]; dcr.
+  assert (PE':PIR2 (ifFstR Equal) (Some ⊝ (getAnn ⊝ als) \\ (fst ⊝ F) ++ DL)
+                ((getAnn ⊝ als ++ Lv) \\ (fst ⊝ F ++ ZL))). {
     rewrite zip_app; eauto with len.
     eapply PIR2_app; eauto using restrict_ifFstR, PIR2_ifFstR_refl.
-    dcr; inv_get.
-    edestruct IHIC1; eauto. econstructor. eauto. eauto. eauto.
-    eauto. reflexivity.
-    econstructor. eauto. eauto. exploit H12; eauto. eapply srd_monotone. eapply H1.
-    (*todo*). simpl in *. dcr.
-    do 2 eexists; split; [|split]; eauto.
-    PIR2_inv. inv_get. exploit H7; eauto; dcr.
-    (*todo*).
-  - edestruct IHIC; eauto. rewrite zip_app; eauto with len.
-    eapply PIR2_app; eauto using restrict_ifFstR, PIR2_ifFstR_refl.
-    destruct l; simpl in *; dcr; inv_get.
-    eauto with cset.
-(*todo*).
-
+  }
+  exploit srd_globals_live; eauto using restrict_ifFstR with len.
+  dcr.
+  setoid_rewrite <- H3. inv_get.
+  simpl in *.
+  edestruct (@get_length_eq _ _ (fst ⊝ F ++ ZL) (getAnn ⊝ als ++ Lv)); eauto.
+  eauto with len.
+  PIR2_inv; inv_get.
+  exploit srd_globals_live_F; eauto using get_app_right, srd_globals_live.
+  dcr. do 2 eexists; split; [|split]; eauto.
+  rewrite H10, H5; eauto.
+Qed.
 
 (** *** On a coherent program a liveness analysis which is sound imperatively is also sound functionally. *)
 
@@ -219,26 +322,29 @@ match goal with
   rewrite (@List.map_app _ _ (restr G) A B)
 end.
 
-Lemma srd_live_functional s ZL Lv DL alv
+Lemma srd_live_functional s ZL Lv DL alv  (Len2 : ❬ZL❭ = ❬Lv❭) (Len3 : ❬ZL❭ = ❬DL❭)
 : live_sound Imperative ZL Lv s alv
   -> srd DL s alv
   -> PIR2 (ifFstR Equal) DL (Lv \\ ZL)
-  -> noUnreachableCode s
+  -> noUnreachableCode isCalled s
   -> live_sound FunctionalAndImperative ZL Lv s alv.
 Proof.
   intros LS SRD PE NUC.
   general induction SRD;
     invt live_sound; invt noUnreachableCode; simpl in * |- *;
       eauto using live_sound, restrict_ifFstR.
-  - econstructor; eauto.
-    + eapply IHSRD; eauto using PIR2_app, restrict_ifFstR, PIR2_ifFstR_refl.
+  - assert(PIR2 (ifFstR Equal) (Some ⊝ (getAnn ⊝ als) \\ (fst ⊝ F) ++ DL)
+                ((getAnn ⊝ als ++ Lv) \\ (fst ⊝ F ++ ZL))). {
+      eauto using PIR2_app, PIR2_ifFstR_refl.
+    }
+    econstructor; eauto.
+    + eapply IHSRD; eauto with len.
     + intros.
-      eapply H1; eauto 10 using PIR2_app, restrict_ifFstR, PIR2_ifFstR_refl.
+      eapply H1; eauto 10 using restrict_ifFstR with len.
     + intros. exploit H12; eauto; dcr.
       simpl; split; eauto.
-      edestruct srd_globals_live as [lv' [Z' ?]];
-        eauto using PIR2_app, restrict_eqReq, PIR2_ifFstR_refl with len.
-      dcr. simpl in *. inv_get.
-      unfold lminus in H17. rewrite H17; eauto.
+      exploit H6; eauto using get_range.
+      edestruct srd_globals_live_From as [lv' [Z' ?]]; eauto with len; dcr.
+      inv_get.
+      rewrite <- H13, <- H19. eauto.
 Qed.
-*)
